x diff
$$
{\exp{\left({\text{const.} \times {\sum_{i, j}\left({{x} - {\mu}}\right)_{[0] = i}{\Lambda}_{[0] = i, [1] = j}\left({{x} - {\mu}}\right)_{[0] = j}}}\right)} \times {\text{const.} \times \left({{\sum_{i, j}{\delta_{[0], [1]}}_{[0] = i}{\Lambda}_{[0] = i, [1] = j}\left({{x} - {\mu}}\right)_{[0] = j}} + {\sum_{i, j}{\delta_{[0], [1]}}_{[0] = i}\left({{x} - {\mu}}\right)_{[0] = j}{\Lambda}_{[0] = j, [1] = i}}}\right)}}
$$
mu diff
$$
{\exp{\left({\text{const.} \times {\sum_{i, j}\left({{x} - {\mu}}\right)_{[0] = i}{\Lambda}_{[0] = i, [1] = j}\left({{x} - {\mu}}\right)_{[0] = j}}}\right)} \times {\text{const.} \times \left({{\sum_{i, j}{\delta_{[0], [1]}}_{[0] = i}{\Lambda}_{[0] = i, [1] = j}\left({{x} - {\mu}}\right)_{[0] = j}} + {\sum_{i, j}{\delta_{[0], [1]}}_{[0] = i}\left({{x} - {\mu}}\right)_{[0] = j}{\Lambda}_{[0] = j, [1] = i}}}\right)}}
$$
sigma diff
$$
{\exp{\left({\text{const.} \times {\sum_{i, j}\left({{x} - {\mu}}\right)_{[0] = i}{\Lambda}_{[0] = i, [1] = j}\left({{x} - {\mu}}\right)_{[0] = j}}}\right)} \times {\text{const.} \times {\sum_{i, j}{\delta_{[0], [2]}} {\delta_{[1], [3]}}_{[0] = i, [1] = j}\left({{x} - {\mu}}\right)_{[0] = i}\left({{x} - {\mu}}\right)_{[0] = j}}}}
$$